HexNotationWord.v
@@ -1,0 +1,7 @@
+Require Export bbv.HexNotation.
+Require Import bbv.WordScope.
+
+Notation "'Ox' a" := (NToWord _ (hex a)) (at level 50).
+
+Goal Ox"41" = WO~1~0~0~0~0~0~1.
+Proof. reflexivity. Qed.
